refinement2 relation

subtyping/refinement.v
@@ -31,8 +31,6 @@ Inductive refinementR (seq: st -> st -> Prop): st -> st -> Prop :=
 
 Definition refinement: st -> st -> Prop := fun s1 s2 => paco2 refinementR bot2 s1 s2.
 
-Notation "x '~<' y" := (refinement x y) (at level 50, left associativity).
-
 Lemma refinementR_mon: monotone2 refinementR.
 Proof. unfold monotone2.
        intros.
@@ -44,4 +42,30 @@ Proof. unfold monotone2.
        - constructor.
 Qed.
 
+(* the second refinement *)
 
+Inductive refinementR2 (seq: st -> st -> Prop): st -> st -> Prop :=
+  | ref2_a  : forall w w' p l s s' a n, subsort s' s ->
+                                        seq w (merge_ap_contn p a w' n)  ->
+                                        act_eq w (merge_ap_contn p a w' n) ->
+                                        refinementR2 seq (st_receive p [(l,s,w)]) (merge_ap_contn p a (st_receive p [(l,s',w')]) n)
+  | ref2_b  : forall w w' p l s s' b n, subsort s s' ->
+                                        seq w (merge_bp_contn p b w' n) ->
+                                        act_eq w (merge_bp_contn p b w' n) ->
+                                        refinementR2 seq (st_send p [(l,s,w)]) (merge_bp_contn p b (st_send p [(l,s',w')]) n)
+  | ref2_end: refinementR2 seq st_end st_end.
+
+Definition refinement2: st -> st -> Prop := fun s1 s2 => paco2 refinementR2 bot2 s1 s2.
+
+Notation "x '~<' y" := (refinement2 x y) (at level 50, left associativity).
+
+Lemma refinementR2_mon: monotone2 refinementR2.
+Proof. unfold monotone2.
+       intros.
+       induction IN; intros.
+       - specialize(ref2_a r'); intro Ha. apply Ha; try easy.
+         apply LE. exact H0.
+       - specialize(ref2_b r'); intro Ha. apply Ha; try easy.
+         apply LE. exact H0.
+       - constructor.
+Qed.
