src/reordering.v
@@ -53,6 +53,10 @@ Inductive coseqIn: (participant * dir) -> coseq (participant * dir) -> Prop :=
   | CoInSplit1 x xs y ys: force xs = cocons y ys -> x = y  -> coseqIn x xs
   | CoInSplit2 x xs y ys: force xs = cocons y ys -> x <> y -> coseqIn x ys -> coseqIn x xs.
 
+Definition act_eq (w w': st) := forall a, coseqIn a (act w) <-> coseqIn a (act w').
+
+Definition act_neq (w w': st) := (exists a, coseqIn a (act w) /\ (coseqIn a (act w') -> False) \/ coseqIn a (act w') /\ (coseqIn a (act w) -> False)).
+
 (* alternative coinductive membership check measures *)
 Inductive coseqInL (R: coseq (participant * dir) -> list (participant * dir) -> Prop): 
                     coseq (participant * dir) -> list (participant * dir) -> Prop :=
@@ -75,157 +79,12 @@ Proof. unfold monotone2.
          apply LE, H0.
 Qed.
 
-Inductive coseqInLI: coseq (participant * dir) -> list (participant * dir) -> Prop :=
-  | ci_nil : forall ys, coseqInLI (Delay conil) ys
-  | ci_incl: forall x xs ys,
-             List.In x ys ->
-             coseqInLI xs ys ->
-             coseqInLI (Delay (cocons x xs)) ys.
-
 Inductive coseqInR: list (participant * dir) -> coseq (participant * dir) -> Prop :=
   | l_nil : forall ys, coseqInR nil ys
   | l_incl: forall x xs ys,
             coseqIn x ys ->
             coseqInR xs ys ->
             coseqInR (x::xs) ys.
-
-Lemma coseqInRInv: forall l w, coseqInR l (act w) -> 
-                              (l = [] \/ (forall x, List.In x l -> coseqIn x (act w))).
-Proof. intros.
-       induction H. left. easy.
-       destruct IHcoseqInR. subst.
-       right. intros a Ha.
-       inversion Ha. subst. easy. easy.
-       right. intros a Ha.
-       inversion Ha. subst. easy.
-       apply H1. easy.
-Qed.
-
-Lemma coseqInRInv2: forall l w,
-  (l = [] \/ (forall x, List.In x l -> coseqIn x (act w))) -> coseqInR l (act w).
-Proof. intros.
-       destruct H. subst. constructor.
-       induction l; intros.
-       - constructor.
-       - constructor. apply H. simpl. left. easy.
-         apply IHl. intros. apply H.
-         simpl. right. easy.
-Qed.
-
-Axiom ext: forall w l, coseqInLC (act w) l -> coseqInLI (act w) l.
-
-Lemma ext_rev: forall w l, coseqInLI (act w) l -> coseqInLC (act w) l.
-Proof. intros.
-       induction H.
-       pfold. constructor.
-       pfold.
-       punfold IHcoseqInLI.
-       inversion IHcoseqInLI.
-       subst. simpl. constructor.
-       easy. left. pfold. easy.
-       subst.
-       constructor. easy.
-       unfold upaco2 in H2. destruct H2.
-       punfold H2. apply coseqInLC_mon.
-       easy.
-       apply coseqInLC_mon.
-Qed.
-
-Lemma liftExt: forall w l, coseqInLI (act w) l -> (forall a, coseqIn a (act w) -> List.In a l).
-Proof. intros.
-       induction H.
-       inversion H0. subst. easy. subst. easy.
-       inversion H0. subst. simpl in H2. inversion H2. subst. easy.
-       subst. simpl in H2. inversion H2. subst. apply IHcoseqInLI. easy.
-Qed.
-
-Lemma extC: forall w l, coseqInLC (act w) l -> (forall a, coseqIn a (act w) -> List.In a l).
-Proof. intros.
-       apply liftExt with (w := w).
-       apply ext. easy. easy.
-Qed.
-
-Lemma coseqInLCInv: forall l w, coseqInLC (act w) l -> 
-                                ((act w) = Delay conil \/ (forall x, coseqIn x (act w) -> List.In x l)).
-Proof. intros.
-       specialize(extC w l H); intro Hax.
-       destruct (act w), force.
-       - left. easy.
-       - right. intros a Ha.
-         punfold H.
-         apply coseqInLC_mon.
-Qed.
-
-Definition act_eq (w w': st) := forall a, coseqIn a (act w) <-> coseqIn a (act w').
-
-Definition act_neq (w w': st) := (exists a, coseqIn a (act w) /\ (coseqIn a (act w') -> False) \/ coseqIn a (act w') /\ (coseqIn a (act w) -> False)).
-
-Lemma coind_ext: forall w1 w2,
-  (exists L1, exists L2, 
-    coseqInLC (act w1) L1 /\ coseqInLC (act w2) L2 /\
-    coseqInR L1 (act w1) /\ coseqInR L2 (act w2) /\ (forall x, List.In x L1 <-> List.In x L2)) -> 
-  act_eq w1 w2.
-Proof. intros w1 w2 (l1,(l2,(Ha,(Hb,(Hc,(Hd,He)))))).
-       unfold act_eq. intro a.
-       split. intro Hf.
-       apply coseqInRInv in Hc, Hd.
-       apply coseqInLCInv in Ha, Hb.
-       destruct Ha as [Ha | Ha].
-       rewrite Ha in Hf.
-       inversion Hf. subst. easy. subst. easy.
-       specialize(Ha a Hf).
-       apply He in Ha.
-       destruct Hd as [Hd | Hd]. subst. easy.
-       apply Hd. easy.
-
-       intro Hf.
-       apply coseqInRInv in Hc, Hd.
-       apply coseqInLCInv in Ha, Hb.
-       destruct Hb as [Hb | Hb].
-       rewrite Hb in Hf.
-       inversion Hf. subst. easy. subst. easy.
-       specialize(Hb a Hf).
-       apply He in Hb.
-       destruct Hc as [Hc | Hc]. subst. easy.
-       apply Hc. easy.
-Qed.
-
-Axiom finAct: forall w1 w2, 
-  act_eq w1 w2 ->
-  (exists L, 
-    coseqInLI (act w1) L /\ (forall x, List.In x L -> coseqIn x (act w1)) /\
-    coseqInLI (act w2) L /\ (forall x, List.In x L -> coseqIn x (act w2))
-   ).
-
-Lemma finiteAct: forall w1 w2, 
-  act_eq w1 w2 ->
-  (exists L1, exists L2,
-    coseqInLC (act w1) L1 /\ coseqInLC (act w2) L2 /\
-    coseqInR L1 (act w1) /\ coseqInR L2 (act w2) /\
-    (forall x, List.In x L1 <-> List.In x L2)
-  ).
-Proof. intros.
-       apply finAct in H.
-       destruct H as (l,(Ha,(Hb,(Hc,Hd)))).
-       exists l.
-       exists l.
-       split. apply ext_rev. exact Ha.
-       split. apply ext_rev. exact Hc.
-       split. apply coseqInRInv2. right. exact Hb.
-       split. apply coseqInRInv2. right. exact Hd.
-       easy.
-Qed.
-
-Lemma mem_ext: forall w1 w2,
-  (exists L1, exists L2,
-    coseqInLC (act w1) L1 /\ coseqInLC (act w2) L2 /\
-    coseqInR L1 (act w1) /\ coseqInR L2 (act w2) /\
-    (forall x, List.In x L1 <-> List.In x L2)
-  ) <-> act_eq w1 w2.
-Proof. split.
-       apply coind_ext.
-       apply finiteAct.
-Qed.
 
 Lemma act_eq_neq: forall w w', (act_eq w w' -> False) -> act_neq w w'.
 Proof. intros.
